\documentclass[uplatex]{jsarticle}
\usepackage[dvipdfmx]{graphicx}
\renewcommand{\baselinestretch}{3}
\begin{document}
初期値問題
\setcounter{section}{17}
\section{}
\begin{eqnarray}
  (9x^2D^2+3xD+I)y&=&0,\hspace{1zw} y(1)=1, y'(1)=0 \\
  9x^2D^2y+3xDy+Iy &=&0 \\
  9x^2y'' +3xy'+y &=&0 
\end{eqnarray}
$$ 9m(m-1)x^m +3mx^m + x^m =0 $$
\begin{eqnarray}
  9m^2 -6m +1 &=&0 \\
  m= \frac{1}{3} \hspace{1zw} 重解
\end{eqnarray}
$$ y_1 = x^{\frac{1}{3}}, \hspace{1zw} y_2 = x^{\frac{1}{3}}logx $$
\begin{eqnarray}
  y &=& x^{\frac{1}{3}}(c_1+c_2lnx) \\ y' &=&\frac{1}{3}(c_1+c_2lnx) +c_2x^{\-frac{2}{3}} 
\end{eqnarray}
$$ c_1 = 1, \hspace{1zw} c_2 = -\frac{1}{3} $$
$$ y = x^{\frac{1}{3}}(1+\frac{1}{3}lnx) $$

\newpage
\includegraphics{./0_100.png}

\includegraphics{./0_7.png}
\section{}
$$ (x^2D^2 -xD -15I)y =0, \hspace{1zw}y(1) = 0.1,y'(1)=-4.5$$
$$ x^2y'' -xy' -15y =0 $$
$$ m (m-1)x^m -mx^m -15x^m =0 $$
$$ m^2 -2m -15 = 0 $$
$$ m = 5, -3 $$
$$ y = c_1x^5 + c_2 x^{-3}, \hspace{1zw} y' = 5c_1x^4 -3 c_2x^{-4} $$
$$ c_1 = -0.525, \hspace{1zw} c_2 = 0.625 $$
$$y = -0.525x^5 + 0.625x^{-3} $$
\end{document}
